src/ocaml/plugin/generated/Pulse_Lib_Core_Typing.ml
@@ -1,46 +1,4 @@
 open Prims
-let (return_post_with_eq :
-  FStar_Reflection_Types.universe ->
-    FStar_Reflection_Types.term ->
-      FStar_Reflection_Types.term ->
-        FStar_Reflection_Types.term ->
-          FStar_Reflection_V2_Data.var -> FStar_Reflection_Types.term)
-  =
-  fun u ->
-    fun a ->
-      fun e ->
-        fun p ->
-          fun x ->
-            let x_tm = FStar_Reflection_Typing.var_as_term x in
-            let eq2_tm = Pulse_Reflection_Util.mk_eq2 u a x_tm e in
-            let p_app_x =
-              FStar_Reflection_V2_Builtins.pack_ln
-                (FStar_Reflection_V2_Data.Tv_App
-                   (p, (x_tm, FStar_Reflection_V2_Data.Q_Explicit))) in
-            let star_tm =
-              Pulse_Reflection_Util.mk_star p_app_x
-                (Pulse_Reflection_Util.mk_pure eq2_tm) in
-            Pulse_Reflection_Util.mk_abs a
-              FStar_Reflection_V2_Data.Q_Explicit
-              (FStar_Reflection_Typing.subst_term star_tm
-                 [FStar_Reflection_Typing.ND (x, Prims.int_zero)])
-let (return_stt_comp :
-  FStar_Reflection_Types.universe ->
-    FStar_Reflection_Types.term ->
-      FStar_Reflection_Types.term ->
-        FStar_Reflection_Types.term ->
-          FStar_Reflection_V2_Data.var -> FStar_Reflection_Types.term)
-  =
-  fun u ->
-    fun a ->
-      fun e ->
-        fun p ->
-          fun x ->
-            Pulse_Reflection_Util.mk_stt_comp u a
-              (FStar_Reflection_V2_Builtins.pack_ln
-                 (FStar_Reflection_V2_Data.Tv_App
-                    (p, (e, FStar_Reflection_V2_Data.Q_Explicit))))
-              (return_post_with_eq u a e p x)
 let (return_stt_noeq_comp :
   FStar_Reflection_Types.universe ->
     FStar_Reflection_Types.term ->
@@ -60,24 +18,6 @@ let (neutral_fv : FStar_Reflection_Types.term) =
     (FStar_Reflection_V2_Data.Tv_FVar
        (FStar_Reflection_V2_Builtins.pack_fv
           Pulse_Reflection_Util.neutral_lid))
-let (return_stt_atomic_comp :
-  FStar_Reflection_Types.universe ->
-    FStar_Reflection_Types.term ->
-      FStar_Reflection_Types.term ->
-        FStar_Reflection_Types.term ->
-          FStar_Reflection_V2_Data.var -> FStar_Reflection_Types.term)
-  =
-  fun u ->
-    fun a ->
-      fun e ->
-        fun p ->
-          fun x ->
-            Pulse_Reflection_Util.mk_stt_atomic_comp neutral_fv u a
-              Pulse_Syntax_Pure.tm_emp_inames
-              (FStar_Reflection_V2_Builtins.pack_ln
-                 (FStar_Reflection_V2_Data.Tv_App
-                    (p, (e, FStar_Reflection_V2_Data.Q_Explicit))))
-              (return_post_with_eq u a e p x)
 let (return_stt_atomic_noeq_comp :
   FStar_Reflection_Types.universe ->
     FStar_Reflection_Types.term ->
@@ -93,24 +33,6 @@ let (return_stt_atomic_noeq_comp :
             (FStar_Reflection_V2_Builtins.pack_ln
                (FStar_Reflection_V2_Data.Tv_App
                   (p, (x, FStar_Reflection_V2_Data.Q_Explicit)))) p
-let (return_stt_ghost_comp :
-  FStar_Reflection_Types.universe ->
-    FStar_Reflection_Types.term ->
-      FStar_Reflection_Types.term ->
-        FStar_Reflection_Types.term ->
-          FStar_Reflection_V2_Data.var -> FStar_Reflection_Types.term)
-  =
-  fun u ->
-    fun a ->
-      fun e ->
-        fun p ->
-          fun x ->
-            Pulse_Reflection_Util.mk_stt_ghost_comp u a
-              Pulse_Syntax_Pure.tm_emp_inames
-              (FStar_Reflection_V2_Builtins.pack_ln
-                 (FStar_Reflection_V2_Data.Tv_App
-                    (p, (e, FStar_Reflection_V2_Data.Q_Explicit))))
-              (return_post_with_eq u a e p x)
 let (return_stt_ghost_noeq_comp :
   FStar_Reflection_Types.universe ->
     FStar_Reflection_Types.term ->
@@ -126,82 +48,7 @@ let (return_stt_ghost_noeq_comp :
             (FStar_Reflection_V2_Builtins.pack_ln
                (FStar_Reflection_V2_Data.Tv_App
                   (p, (x, FStar_Reflection_V2_Data.Q_Explicit)))) p
-let (while_typing :
-  FStar_Reflection_Types.env ->
-    FStar_Reflection_Types.term ->
-      FStar_Reflection_Types.term ->
-        FStar_Reflection_Types.term ->
-          (unit, unit, unit) FStar_Reflection_Typing.tot_typing ->
-            (unit, unit, unit) FStar_Reflection_Typing.tot_typing ->
-              (unit, unit, unit) FStar_Reflection_Typing.tot_typing ->
-                (unit, unit, unit) FStar_Reflection_Typing.tot_typing)
-  =
-  fun g ->
-    fun inv ->
-      fun cond ->
-        fun body -> fun uu___ -> fun uu___1 -> fun uu___2 -> Prims.admit ()
-let (par_post :
-  FStar_Reflection_Types.universe ->
-    FStar_Reflection_Types.term ->
-      FStar_Reflection_Types.term ->
-        FStar_Reflection_Types.term ->
-          FStar_Reflection_Types.term ->
-            FStar_Reflection_V2_Data.var -> FStar_Reflection_Types.term)
-  =
-  fun u ->
-    fun aL ->
-      fun aR ->
-        fun postL ->
-          fun postR ->
-            fun x ->
-              let x_tm = FStar_Reflection_Typing.var_as_term x in
-              let postL1 =
-                FStar_Reflection_V2_Builtins.pack_ln
-                  (FStar_Reflection_V2_Data.Tv_App
-                     (postL,
-                       ((Pulse_Reflection_Util.mk_fst u u aL aR x_tm),
-                         FStar_Reflection_V2_Data.Q_Explicit))) in
-              let postR1 =
-                FStar_Reflection_V2_Builtins.pack_ln
-                  (FStar_Reflection_V2_Data.Tv_App
-                     (postR,
-                       ((Pulse_Reflection_Util.mk_snd u u aL aR x_tm),
-                         FStar_Reflection_V2_Data.Q_Explicit))) in
-              let post = Pulse_Reflection_Util.mk_star postL1 postR1 in
-              FStar_Reflection_Typing.subst_term post
-                [FStar_Reflection_Typing.ND (x, Prims.int_zero)]
-let (elim_exists_post_body :
-  FStar_Reflection_Types.universe ->
-    FStar_Reflection_Types.term ->
-      FStar_Reflection_Types.term ->
-        FStar_Reflection_V2_Data.var -> FStar_Reflection_Types.term)
-  =
-  fun u ->
-    fun a ->
-      fun p ->
-        fun x ->
-          let x_tm = FStar_Reflection_Typing.var_as_term x in
-          let reveal_x = Pulse_Reflection_Util.mk_reveal u a x_tm in
-          let post =
-            FStar_Reflection_V2_Builtins.pack_ln
-              (FStar_Reflection_V2_Data.Tv_App
-                 (p, (reveal_x, FStar_Reflection_V2_Data.Q_Explicit))) in
-          FStar_Reflection_Typing.subst_term post
-            [FStar_Reflection_Typing.ND (x, Prims.int_zero)]
-let (elim_exists_post :
-  FStar_Reflection_Types.universe ->
-    FStar_Reflection_Types.term ->
-      FStar_Reflection_Types.term ->
-        FStar_Reflection_V2_Data.var -> FStar_Reflection_Types.term)
-  =
-  fun u ->
-    fun a ->
-      fun p ->
-        fun x ->
-          let erased_a = Pulse_Reflection_Util.mk_erased u a in
-          Pulse_Reflection_Util.mk_abs erased_a
-            FStar_Reflection_V2_Data.Q_Explicit
-            (elim_exists_post_body u a p x)
+
 let intro_exists_erased_typing :
   'uuuuu 'uuuuu1 'uuuuu2 'uuuuu3 . 'uuuuu -> 'uuuuu1 -> 'uuuuu2 -> 'uuuuu3 =
   fun uu___ -> fun uu___1 -> fun uu___2 -> Prims.admit ()
