src/ocaml/plugin/generated/Pulse_Typing_Combinators.ml
@@ -3712,11 +3712,7 @@ let (apply_frame :
                          (res_typing, pre_typing, x, post_typing) ->
                          let st_equiv =
                            Pulse_Typing.ST_SLPropEquiv
-                             (g, c', c'', x, (), (), (),
-                               (FStar_Reflection_Typing.Rel_refl
-                                  ((Pulse_Typing.elab_env g),
-                                    (Pulse_Syntax_Base.comp_res c'),
-                                    FStar_Reflection_Typing.R_Eq)), (), ()) in
+                             (g, c', c'', x, (), (), (), (), (), ()) in
                          let t_typing2 =
                            Pulse_Typing.T_Equiv
                              (g, t, (Pulse_Typing.add_frame c frame), c'',
