src/ocaml/plugin/generated/Pulse_Typing_Metatheory_Base.ml
@@ -232,13 +232,7 @@ let (st_equiv_weakening :
                   Pulse_Typing.ST_SLPropEquiv
                     ((Pulse_Typing_Env.push_env
                         (Pulse_Typing_Env.push_env g g1) g'), c11, c21, x,
-                      (), (), (),
-                      (FStar_Reflection_Typing.Rel_refl
-                         ((Pulse_Typing.elab_env
-                             (Pulse_Typing_Env.push_env
-                                (Pulse_Typing_Env.push_env g g1) g')),
-                           (Pulse_Syntax_Base.comp_res c11),
-                           FStar_Reflection_Typing.R_Eq)), (), ())
+                      (), (), (), (), (), ())
 
 let rec (st_sub_weakening :
   Pulse_Typing_Env.env ->
@@ -768,15 +762,7 @@ let (st_equiv_subst :
                               (Pulse_Typing_Env.subst_env g' (nt x e))),
                             (Pulse_Syntax_Naming.subst_comp c11 (nt x e)),
                             (Pulse_Syntax_Naming.subst_comp c21 (nt x e)), y,
-                            (), (), (),
-                            (FStar_Reflection_Typing.Rel_refl
-                               ((Pulse_Typing.elab_env
-                                   (Pulse_Typing_Env.push_env g
-                                      (Pulse_Typing_Env.subst_env g' (nt x e)))),
-                                 (Pulse_Syntax_Base.comp_res
-                                    (Pulse_Syntax_Naming.subst_comp c11
-                                       (nt x e))),
-                                 FStar_Reflection_Typing.R_Eq)), (), ())
+                            (), (), (), (), (), ())
 let (st_comp_typing_subst :
   Pulse_Typing_Env.env ->
     Pulse_Syntax_Base.var ->
